Veir.lean
@@ -17,6 +17,9 @@ import Veir.Interfaces.ControlFlowInterfaces
 import Veir.Passes.ArithToLLVM.Proofs
 import Veir.Passes.Canonicalize.Proofs
 import Veir.Passes.RISCVCombines.Proofs
+import Veir.Dialects.LLZK.Semantics.Constraint
+import Veir.Dialects.LLZK.Analysis.RangeAnalysisProofs
+import Veir.Passes.LLZK.DedupConstraintsProofs
 import Veir.Benchmarks
 import Veir.Parser.Lexer
 import Veir.Interpreter
